% ./equations/energy-kinetic-vs-mass.tex
% ============================================================================ %
\documentclass[../main.tex]{subfiles}%
\begin{document}%
% ============================================================================ %
    \Xequation%    
    % ======================================================================== %
    \begin{equation}%
        (E_{c} + E_{d}) - (E_{a} + E_{b})
        =%
        [(m_{c} + m_{d}) - (m_{a} + m_{b})] c^{2}%
        \label{eq:energy-kinetic-vs-mass}%
    \end{equation}%
% ============================================================================ %
\end{document}%