% ./equations/mosaic-stitch-composite.tex
% ============================================================================ %
\documentclass[../main.tex]{subfiles}%
\begin{document}%
% ============================================================================ %
    \Xequation%    
    % ======================================================================== %
    \begin{equation*}%
        h(x,y) = F^{*}(x,y) \cdot [G^{*}(x,y)]^{-1}
    \end{equation*}%
    % ======================================================================== %
    \par%
    % ======================================================================== %
    \begin{equation}%
        h(x,y) =%
        \sum^{K}_{i=1}%
        f^{*}_{i}(x,y)%
        \cdot%
        \left[%
        \sum^{K}_{i=1}%
        g^{*}_{i}(x,y)%
        \right]^{-1}%
        \label{eq:mosaic-stitch-composite}%  
    \end{equation}%  
% ============================================================================ %
\end{document}%