% ./equations/mosaic-stitch-shifted-function.tex
% ============================================================================ %
\documentclass[../main.tex]{subfiles}%
\begin{document}%
% ============================================================================ %
    \Xequation%    
    % ======================================================================== %
    \begin{equation*}%
        f_{i}^{*}(x,y)%
        =%
        f_{i}(x+\Delta x_{i},y+\Delta y_{i})%
    \end{equation*}%
    % ======================================================================== %
    \par%
    % ======================================================================== %
    \begin{equation}%
        f_{i}^{*}(x,y) =%
        \begin{bmatrix}%
            f_{i}(1+\Delta x_{i},1+\Delta y_{i}) && f_{i}(1+\Delta x_{i},2+\Delta y_{i}) && \dots && f_{i}(1+\Delta x_{i},N+\Delta y_{i}) \\%
            f_{i}(2+\Delta x_{i},1+\Delta y_{i}) && f_{i}(2+\Delta x_{i},2+\Delta y_{i}) && \dots && f_{i}(2+\Delta x_{i},N+\Delta y_{i}) \\%
            \vdots && \vdots && \ddots && \vdots \\%
            f_{i}(M+\Delta x_{i},1+\Delta y_{i}) && f_{i}(M+\Delta x_{i},2+\Delta y_{i}) && \dots && f_{i}(M+\Delta x_{i},N+\Delta y_{i}) \\%
        \end{bmatrix}%
        \label{eq:mosaic-stitch-shifted-function}%
    \end{equation}%     
% ============================================================================ %
\end{document}%